Reformulate

lean/language.lean
@@ -11,13 +11,11 @@ import tactic.ring_exp
 import tactic.tidy
 import tactic.where
 
-/-! # Incorrectness logic library -/
-
-namespace IncLoLib
-
-meta def tactic.dec_trivial := `[exact dec_trivial]
+namespace IncLoLang
 
 /-! ## State-/
+
+meta def tactic.dec_trivial := `[exact dec_trivial]
 
 def state : Type := string -> ℕ
 
@@ -33,9 +31,8 @@ begin
        ...                = val : by finish,
 end
 
-
-@[simp] lemma update_apply_ne (name name' : string) (val : ℕ) (s : state)
-    (h : name' ≠ name . tactic.dec_trivial) :
+@[simp] lemma update_apply_ne (name name' : string) (val : ℕ) (s : state) 
+  (h : name' ≠ name . tactic.dec_trivial) : 
     s{name ↦ val} name' = s name' :=
 begin
   calc s{name ↦ val} name' = (λname', if name' = name then val else s name') name' : by refl
@@ -56,6 +53,7 @@ inductive stmt : Type
 | skip   : stmt
 | assign : string → (state → ℕ) → stmt
 | seq    : stmt → stmt → stmt
+| error    : stmt
 -- | ite    : (state → Prop) → stmt → stmt → stmt
 -- | while  : (state → Prop) → stmt → stmt
 
@@ -64,6 +62,7 @@ def eval : option state -> stmt -> option state
 | none (stmt.assign v s)        := none
 | (some st) (stmt.assign v s)   := st{v ↦ s st}
 | st (stmt.seq n m)             := (eval (eval st n) m)
+| st (stmt.error)             := none
 
 infixr ` ;; ` : 90 := stmt.seq
 
@@ -77,46 +76,6 @@ infixr ` ;; ` : 90 := stmt.seq
 #eval option.bind (eval (none)
   ((stmt.assign "x" (λ s, 1 + s "y")) ;; 
    (stmt.assign "x" (λ s, 1 + s "x")))) (λ s, some (s "x"))
+#eval option.bind (eval (some (λ x, 0)) stmt.error) (λ s, some (s "x"))
 
-/-! ## Big step semantics -/
-
-inductive big_step : stmt × option state → option state → Prop
-| skip {s} :
-  big_step (stmt.skip, s) s
-| assign {x f s} :
-  big_step (stmt.assign x f, some s) (some (s{x ↦ f s}))
-| seq {S T s t u} (hS : big_step (S, s) t)
-    (hT : big_step (T, t) u) :
-  big_step (S ;; T, s) u
--- | ite_true {b : state → Prop} {S T s t} (hcond : b s)
---     (hbody : big_step (S, s) t) :
---   big_step (stmt.ite b S T, s) t
--- | ite_false {b : state → Prop} {S T s t} (hcond : ¬ b s)
---     (hbody : big_step (T, s) t) :
---   big_step (stmt.ite b S T, s) t
--- | while_true {b : state → Prop} {S s t u} (hcond : b s)
---     (hbody : big_step (S, s) t)
---     (hrest : big_step (stmt.while b S, t) u) :
---   big_step (stmt.while b S, s) u
--- | while_false {b : state → Prop} {S s} (hcond : ¬ b s) :
---   big_step (stmt.while b S, s) s
-
-infix ` ⟹ ` : 110 := big_step
-
-/-! ## Hoare Logic -/
-
-def partial_hoare (P : option state → Prop) (S : stmt)
-  (Q : option state → Prop) : Prop := 
-  ∀ s t, (P s → (S, s) ⟹ t) → Q t
-
-notation `{* ` P : 1 ` *} ` S : 1 ` {* ` Q : 1 ` *}` :=
-  partial_hoare
-
-namespace hoare_logic
-
-
-
-end hoare_logic
-
-
-end IncLoLib
+end IncLoLang
