lean/incorrectness_logic.lean
@@ -1,0 +1,76 @@
+
+import algebra
+import data.real.basic
+import data.vector
+import tactic.explode
+import tactic.find
+import tactic.induction
+import tactic.linarith
+import tactic.rcases
+import tactic.rewrite
+import tactic.ring_exp
+import tactic.tidy
+import tactic.where
+
+import lean.language
+
+namespace IncLoIncorrectness
+
+inductive LogicType : Type
+| er
+| ok
+
+inductive post: IncLoLang.stmt -> LogicType -> (IncLoLang.state) -> (IncLoLang.state) -> Prop
+| seq_er {S T s t u} (H1: post S LogicType.ok s t) (H2: post T LogicType.er t u) : /- TODO: This needs to use post norm instead? How to encode? -/
+  post (S ;; T) LogicType.er s u
+| error {s}:
+  post IncLoLang.stmt.error LogicType.er s s
+| skip {s} :
+  post IncLoLang.stmt.skip LogicType.ok s s
+| assign {x s f} :
+  post (IncLoLang.stmt.assign x f) LogicType.ok s (s{x ↦ (f s)})
+| seq_ok {S T s t u} (H1: post S LogicType.ok s t) (H2: post T LogicType.ok t u) :
+  post(S ;; T) LogicType.ok s u
+
+def incorrectness_logic (ty: LogicType) (P : (IncLoLang.state) → Prop) (R : IncLoLang.stmt)
+  (Q : (IncLoLang.state) → Prop) : Prop := 
+  ∀ s t, Q s -> post R ty t s -> P t
+
+def hoare_logic (ty: LogicType) (P : (IncLoLang.state) → Prop) (R : IncLoLang.stmt)
+  (Q : (IncLoLang.state) → Prop) : Prop := 
+  ∀ s t, P s -> post R ty t s -> Q t
+
+notation `{* ` P : 1 ` *} ` S : 1 ` {* ` Q : 1 ` *}` ty: 2 :=
+  hoare_logic ty P S Q
+
+notation `[* ` P : 1 ` *] ` S : 1 ` [* ` Q : 1 ` *]` ty: 2 :=
+  hoare_logic ty P S Q
+
+lemma hoare_skip_intro_ok { P: IncLoLang.state -> Prop } : {* P *} IncLoLang.stmt.skip {* P *} LogicType.ok:=
+begin
+  intros s t hs hst,
+  cases hst,
+  assumption,
+end
+
+lemma hoare_skip_intro_er { P: IncLoLang.state -> Prop } : {* P *} IncLoLang.stmt.skip {* P *} LogicType.er :=
+begin
+  intros s t hs hst,
+  cases hst,
+end
+
+
+lemma inc_skip_intro_ok { P: IncLoLang.state -> Prop } : [* P *] IncLoLang.stmt.skip [* P *] LogicType.ok:=
+begin
+  intros s t hs hst,
+  cases hst,
+  assumption,
+end
+
+lemma inc_skip_intro_er { P: IncLoLang.state -> Prop } : [* P *] IncLoLang.stmt.skip [* P *] LogicType.er :=
+begin
+  intros s t hs hst,
+  cases hst,
+end
+
+end IncLoIncorrectness
